pulse/lib/steel/pulse/Pulse.Soundness.Bind.fsti
@@ -95,3 +95,13 @@ val ghost_bind_typing
   : GTot (RT.tot_typing (elab_env g)
                         (elab_st_typing d)
                         (elab_comp c))
+
+val bind_fn_typing
+  (#g:stt_env)
+  (#t:st_term)
+  (#c:comp)
+  (d:st_typing g t c{T_BindFn? d})
+  (soundness:soundness_t d)
+  : GTot (RT.tot_typing (elab_env g)
+                        (elab_st_typing d)
+                        (elab_comp c))
