pulse/lib/steel/pulse/Pulse.Typing.LN.fst
@@ -1160,6 +1160,12 @@ let rec st_typing_ln (#g:_) (#t:_) (#c:_)
       open_st_term_ln e2 x;
       bind_comp_ln bc
 
+    | T_BindFn _g _e1 e2 _c1 _c2 _b x d1 _u dc1 d2 _u2 c ->
+      st_typing_ln d1;
+      tot_or_ghost_typing_ln dc1;
+      st_typing_ln d2;
+      open_st_term_ln e2 x;
+      comp_typing_ln c
 
     | T_TotBind _ _ _ _ _ _ _ _ _
     | T_GhostBind _ _ _ _ _ _ _ _ _ _ ->
